MCequiv: push post meeting

Exercises/MCequivScript.sml
@@ -1,4 +1,5 @@
 open HolKernel Parse boolLib bossLib;
+open basicSizeTheory;
 
 val _ = new_theory "MCequiv";
 
@@ -13,7 +14,7 @@ Datatype:
           | Less expr expr | Equal expr expr
           | Divide expr expr | If expr expr expr
           | Apply expr expr
-          | Lam
+          | Lam type expr
           | Var num
           | Recfun type type (expr -> expr -> expr)
 End
@@ -23,8 +24,9 @@ Datatype:
 	expr =  Lit bool | Equal expr expr
 		  | If expr expr expr
           | Apply expr expr
-          | Lam expr
-          | Var num
+          | Lam type expr (* TODO: could change type to expr using typetag *)
+          | Var type num (* TODO: remove type here and add a context that carries the mapping from the variables/numbers to their types *)
+          | TypeTag type
 End
 
 val _ = export_rewrites ["expr_size_def"]
@@ -35,19 +37,56 @@ val _ = export_rewrites ["expr_size_def"]
   -----------------
 *)
 
+Definition isVal:
+	(isVal (Lit _) ⇔ T)
+End
+
 Definition isAtom:
 (*	(isAtom (Num _) ⇔ T) ∧ *)
 	(isAtom (Lit _) ⇔ T) ∧
 (*	isAtom (Recfun _ _ _) ∧ *)
-	(isAtom (Var _) ⇔ T) ∧
-	(isAtom (Lam _) ⇔ T) ∧
+	(isAtom (Var _ _) ⇔ T) ∧
+	(isAtom (Lam _ _ _) ⇔ T) ∧
 	(isAtom _ ⇔ F)
 End
 
+Theorem non_atoms_not_isAtom[simp]:
+	¬(isAtom (Equal e1 e2)) ∧
+	¬(isAtom (If e1 e2 e3)) ∧
+	¬(isAtom (Apply e1 e2))
+Proof
+	simp[isAtom]
+QED
+
+(*
+Theorem litIsAtom[simp]:
+	isAtom (Lit a)
+Proof
+	simp[isAtom]
+QED
+
+Theorem varIsAtom[simp]:
+	isAtom (Var a)
+Proof
+	simp[isAtom]
+QED
+*)
+
+
 Definition isVar:
-	(isVar (Var _) ⇔ T) ∧
+	(isVar (Var _ _) ⇔ T) ∧
 	(isVar _ ⇔ F)
 End
+
+Theorem non_var_not_isVar[simp]:
+	¬(isVar (Equal e1 e2)) ∧
+	¬(isVar (If e1 e2 e3)) ∧
+	¬(isVar (Apply e1 e2)) ∧
+	¬(isVar (Lam t1 t2 e1)) ∧
+	¬(isVar (Lit b))
+Proof
+	rw[isVar]
+QED
 
 (*
 Definition M_step:
@@ -77,14 +116,19 @@ End
 *)
 
 Definition subst:
-	subst e1 e2 n = if (isAtom e1 ∧ ¬(isVar e1)) then e1 else case e1 of
+(* TODO: use Lit directly *)
+	subst e1 e2 n = if (isVal e1) then e1 else case e1 of
 		Equal a b => Equal (subst a e2 n) (subst b e2 n)
 	  | If g a b => If (subst g e2 n) (subst a e2 n) (subst b e2 n)
 	  | Apply a b => Apply (subst a e2 n) (subst b e2 n)
-	  | Lam e => Lam (subst e e2 (n+1))
-	  | Var m => if (n = m) then e2 else (Var m)
+	  | Lam t1 t2 e => Lam t1 t2 (subst e e2 (n+1))
+	  | Var t m => if (n = m) then e2 else (Var t m)
 End
 
+(* (\x (\y. xy)) (Var 0) *)
+(* TODO:
+	1. check capture avoiding substitution
+	2. check higher order abstract syntax *)
 
 Definition M_step:
 (*	M_step (Plus (Num a) (Num b)) = Num (a + b) ∧
@@ -102,17 +146,23 @@ Definition M_step:
 	M_step (Divide (Num a) (Num b)) = Num (a `div` b) ∧
 	M_step (Divide (Num a) b) = Divide (Num a) (M_step b) ∧
 	M_step (Divide a b) = Divide (M_step a) b ∧ *)
+	M_step (Lit e) = Lit e ∧
+	M_step (Var t v) = Var t v ∧
+	M_step (Lam t1 t2 e) = Lam t1 t2 e ∧
 	M_step (Equal (Lit a) (Lit b)) = Lit (a = b) ∧
+(*	M_step (Equal (Lit a) (Lam b)) = Lit False ∧
+	M_step (Equal (Lit a) (Var t b)) = Lit False ∧ *)
 	M_step (Equal (Lit a) b) = Equal (Lit a) (M_step b) ∧
+(*	M_step (Equal (Lam a) (Lit b) = Lit False *)
 	M_step (Equal a b) = Equal (M_step a) b ∧
 	M_step (If (Lit True) t e) = t ∧
 	M_step (If (Lit False) t e) = e ∧
 	M_step (If b t e) = If (M_step b) t e ∧
-	(M_step (Apply (Lam e) e2) =
+	(M_step (Apply (Lam t1 t2 e) e2) =
 		if isAtom e2 then
 			subst e e2 0
 		else
-			Apply (Lam e) (M_step e2))	∧
+			Apply (Lam t1 t2 e) (M_step e2))	∧
 	M_step (Apply e1 e2) = Apply (M_step e1) e2
 (*	M_step (Apply rec@(Recfun _ _ f) e2)
 	  | isAtom e2 = f rec e2
@@ -121,12 +171,31 @@ Definition M_step:
 *)
 End
 
+(* TODO *)
+(*
+	e = M_step (Equal e1 e2) ==>
+	?b. e = Lit b \/
+	?e2'. e = ...
+*)
+
+Theorem M_step_equal_bool_or_equal:
+∀e1 e2. (∃b. M_step (Equal e1 e2) = Lit b) ∨
+		(∃e2'. M_step (Equal e1 e2) = Equal e1 e2') ∨
+		(∃e1'. M_step (Equal e1 e2) = Equal e1' e2)
+Proof
+	ho_match_mp_tac M_step_ind >> rw[M_step] >>
+	Cases_on `e2` >> rw[M_step]
+QED
+
+(* TODO; check isabelle/hol: induct cases gives all theorems like above *)
+
 Theorem equal_step_size:
 	∀e1 e2. expr_size (M_step (Equal e1 e2)) < expr_size e1 + (expr_size e2 + 1)
 Proof
 	Cases_on `e1` >>
 QED
 
+(*
 Definition run_M_step:
 	run_M_step e =
 		if isAtom e
@@ -137,9 +206,91 @@ Termination
 	WF_REL_TAC `measure expr_size` >>
 	Induct_on `e` >> rw[isAtom]
 	>- (rename [`expr_size (M_step (Equal e1 e2)) < _`] >>
-		rw[] >> Cases_on `e1` >> Cases_on `e2` >> rw[M_step])
+		rw[] >> Cases_on `e1` >> Cases_on `e2` >> fs[M_step, bool_size_def]
+		>- ())
+End
+*)
+
+(* need to progress + preservation *)
+
+(* expr -> SOME type *)
+Definition typeCheck:
+(*	typeCheck (Num n) = IntTy ∧ *)
+	typeCheck (Lit b) = SOME BoolTy ∧
+(*	typeCheck (Plus e1 e2) = case (typeCheck e1, typeCheck e2) of
+	                           (IntTy, IntTy) -> IntTy
+	                           _ -> error "type error"
+	typeCheck (Minus e1 e2) = case (typeCheck e1, typeCheck e2) of
+	                           (IntTy, IntTy) -> IntTy
+	                           _ -> error "type error"
+	typeCheck (Divide e1 e2) = case (typeCheck e1, typeCheck e2) of
+	                           (IntTy, IntTy) -> IntTy
+	                           _ -> error "type error"
+	typeCheck (Less e1 e2) = case (typeCheck e1, typeCheck e2) of
+	                           (IntTy, IntTy) -> BoolTy
+	                           _ -> error "type error" *)
+	(typeCheck (Equal e1 e2) = case (typeCheck e1, typeCheck e2) of
+	                        (*   (IntTy, IntTy) -> BoolTy *)
+	                         |  (SOME BoolTy, SOME BoolTy) => SOME BoolTy
+	                         |  _ => NONE (* error "type error" *)) ∧
+	(typeCheck (If c t e) = case (typeCheck c, typeCheck t, typeCheck e) of
+	   | (SOME BoolTy, tt, te) => if tt = te then tt else NONE (* error "Branches have different types" *)
+	   | _ => NONE (* error "if condition should be bool" *)) ∧
+	(typeCheck (Apply e1 e2) = case (typeCheck e1, typeCheck e2) of
+	   | (SOME (FunTy t1 t2), SOME t1') => if t1 = t1' then (SOME t2)
+	                                  else NONE (* error "Argument doesn't match function" *)
+	   | _ => NONE) ∧ (* error "Can't apply a non-function" *)
+	typeCheck (Lam t1 t2 e) = SOME (FunTy t1 t2) ∧ (* error "Function body doesn't match type signature" *)
+	typeCheck (Var t n) = SOME t ∧
+	typeCheck (TypeTag t) = SOME t
 End
 
+
+Theorem typeCheck_equal_bool_or_none:
+∀e1 e2.	typeCheck (Equal e1 e2) = SOME BoolTy ∨
+		typeCheck (Equal e1 e2) = NONE
+Proof
+	rw[] >> Cases_on `typeCheck e1` >> Cases_on `typeCheck e2` >> gs[typeCheck]
+	>> Cases_on `x` >> gs[] >> Cases_on `x'` >> gs[]
+QED
+
+Theorem M_progress:
+	∀e t. typeCheck e = SOME t ⇒ isAtom e ∨ ∃e'. M_step e = e'
+Proof
+	rw[M_step]
+QED
+
+Theorem M_preservation:
+	∀e e' t. typeCheck e = SOME t ∧ M_step e = e' ⇒ typeCheck e' = SOME t
+Proof
+	Induct_on `e` >> rw[M_step] >> rw[]
+	>- (Cases_on `e` >> Cases_on `e'` >> rw[M_step]
+		>- rw[typeCheck]
+		>- (fs[typeCheck] >> Cases_on `typeCheck e` >> Cases_on `typeCheck e0` >> gs[]
+			>- (Cases_on `x` >> gs[])
+			>> Cases_on `x` >> gs[] >> Cases_on `x'` >> gs[] >>
+			Cases_on `t''` >> gs[]
+			>- (rename [`typeCheck (M_step (Equal e1 e2)) = SOME IntTy`] >>
+				`(∃b. M_step (Equal e1 e2) = Lit b) ∨
+			     (∃e2'. M_step (Equal e1 e2) = Equal e1 e2') ∨
+			      ∃e1'. M_step (Equal e1 e2) = Equal e1' e2`
+			      	by metis_tac[M_step_equal_bool_or_equal]
+			    >- fs[typeCheck] >> gs[]
+		    	>> rename [`typeCheck (Equal a b) = SOME IntTy`] >>
+		        `typeCheck (Equal a b) = SOME BoolTy ∨ typeCheck (Equal a b) = NONE`
+		        	by metis_tac[typeCheck_equal_bool_or_none] >> fs[])
+			>> rename [`typeCheck (M_step (Equal e1 e2)) = SOME (FunTy t1 t2)`] >>
+			`(∃b. M_step (Equal e1 e2) = Lit b) ∨
+		     (∃e2'. M_step (Equal e1 e2) = Equal e1 e2') ∨
+		      ∃e1'. M_step (Equal e1 e2) = Equal e1' e2`
+			      	by metis_tac[M_step_equal_bool_or_equal]
+			>- fs[typeCheck] >> gs[]
+	    	>> rename [`typeCheck (Equal a b) = SOME (FunTy t1 t2)`] >>
+	        `typeCheck (Equal a b) = SOME BoolTy ∨ typeCheck (Equal a b) = NONE`
+	        	by metis_tac[typeCheck_equal_bool_or_none] >> fs[])
+		>- ()
+		)
+QED
 
 (*
   -----------------
@@ -149,6 +300,16 @@ End
 
 Datatype:
 	value = IntV int | BoolV bool | FunV (expr -> expr -> expr)
+End
+
+Datatype:
+	frame =  PlusF1 expr | PlusF2 value
+           | MinusF1 expr | MinusF2 value
+           | LessF1 expr | LessF2 value
+           | EqualF1 expr | EqualF2 value
+           | DivideF1 expr | DivideF2 value
+           | IfF expr expr
+           | ApplyF1 expr | ApplyF2 value
 End
 
 Datatype:
